@prefix dc: <http://purl.org/dc/elements/1.1/> .
@prefix ns1: <http://ontology.gaming.network/universal/gaming#> .
@prefix owl: <http://www.w3.org/2002/07/owl#> .
@prefix rdf: <http://www.w3.org/1999/02/22-rdf-syntax-ns#> .
@prefix rdfs: <http://www.w3.org/2000/01/rdf-schema#> .
@prefix skos: <http://www.w3.org/2004/02/skos/core#> .
@prefix xsd: <http://www.w3.org/2001/XMLSchema#> .

<http://ontology.gaming.network/core#Actor> a owl:Class ;
    rdfs:comment "DEPRECATED legacy IRI. Use 'http://ontology.gaming.network/universal/gaming#Actor' instead."@en ;
    owl:deprecated true ;
    owl:equivalentClass ns1:Actor .

<http://ontology.gaming.network/core#AdEvent> a owl:Class ;
    rdfs:comment "DEPRECATED legacy IRI. Use 'http://ontology.gaming.network/universal/gaming#AdEvent' instead."@en ;
    owl:deprecated true ;
    owl:equivalentClass ns1:AdEvent .

<http://ontology.gaming.network/core#AdInteraction> a owl:Class ;
    rdfs:comment "DEPRECATED legacy IRI. Use 'http://ontology.gaming.network/universal/gaming#AdInteraction' instead."@en ;
    owl:deprecated true ;
    owl:equivalentClass ns1:AdInteraction .

<http://ontology.gaming.network/core#AtRisk> a owl:Class ;
    rdfs:comment "DEPRECATED legacy IRI. Use 'http://ontology.gaming.network/universal/gaming#AtRisk' instead."@en ;
    owl:deprecated true ;
    owl:equivalentClass ns1:AtRisk .

<http://ontology.gaming.network/core#AttributedInstall> a owl:Class ;
    rdfs:comment "DEPRECATED legacy IRI. Use 'http://ontology.gaming.network/universal/gaming#AttributedInstall' instead."@en ;
    owl:deprecated true ;
    owl:equivalentClass ns1:AttributedInstall .

<http://ontology.gaming.network/core#Bid> a owl:Class ;
    rdfs:comment "DEPRECATED legacy IRI. Use 'http://ontology.gaming.network/universal/gaming#Bid' instead."@en ;
    owl:deprecated true ;
    owl:equivalentClass ns1:Bid .

<http://ontology.gaming.network/core#Campaign> a owl:Class ;
    rdfs:comment "DEPRECATED legacy IRI. Use 'http://ontology.gaming.network/universal/gaming#Campaign' instead."@en ;
    owl:deprecated true ;
    owl:equivalentClass ns1:Campaign .

<http://ontology.gaming.network/core#Churned> a owl:Class ;
    rdfs:comment "DEPRECATED legacy IRI. Use 'http://ontology.gaming.network/universal/gaming#Churned' instead."@en ;
    owl:deprecated true ;
    owl:equivalentClass ns1:Churned .

<http://ontology.gaming.network/core#Device> a owl:Class ;
    rdfs:comment "DEPRECATED legacy IRI. Use 'http://ontology.gaming.network/universal/gaming#Player' instead."@en ;
    owl:deprecated true ;
    owl:equivalentClass ns1:Player .

<http://ontology.gaming.network/core#Dolphin> a owl:Class ;
    rdfs:comment "DEPRECATED legacy IRI. Use 'http://ontology.gaming.network/universal/gaming#Dolphin' instead."@en ;
    owl:deprecated true ;
    owl:equivalentClass ns1:Dolphin .

<http://ontology.gaming.network/core#EngagementLevel> a owl:Class ;
    rdfs:comment "DEPRECATED legacy IRI. Use 'http://ontology.gaming.network/universal/gaming#EngagementLevel' instead."@en ;
    owl:deprecated true ;
    owl:equivalentClass ns1:EngagementLevel .

<http://ontology.gaming.network/core#Event> a owl:Class ;
    rdfs:comment "DEPRECATED legacy IRI. Use 'http://ontology.gaming.network/universal/human_behavior#BehavioralEvent' instead."@en ;
    owl:deprecated true ;
    owl:equivalentClass <http://ontology.gaming.network/universal/human_behavior#BehavioralEvent> .

<http://ontology.gaming.network/core#Game> a owl:Class ;
    rdfs:comment "DEPRECATED legacy IRI. Use 'http://ontology.gaming.network/universal/gaming#Game' instead."@en ;
    owl:deprecated true ;
    owl:equivalentClass ns1:Game .

<http://ontology.gaming.network/core#GameEvent> owl:equivalentClass ns1:GameEvent .

<http://ontology.gaming.network/core#GameSession> a owl:Class ;
    rdfs:comment "DEPRECATED legacy IRI. Use 'http://ontology.gaming.network/universal/gaming#GameSession' instead."@en ;
    owl:deprecated true ;
    owl:equivalentClass ns1:GameSession .

<http://ontology.gaming.network/core#HighEngagement> a owl:Class ;
    rdfs:comment "DEPRECATED legacy IRI. Use 'http://ontology.gaming.network/universal/gaming#HighEngagement' instead."@en ;
    owl:deprecated true ;
    owl:equivalentClass ns1:HighEngagement .

<http://ontology.gaming.network/core#Human> a owl:Class ;
    rdfs:comment "DEPRECATED legacy IRI. Use 'http://ontology.gaming.network/universal/gaming#Human' instead."@en ;
    owl:deprecated true ;
    owl:equivalentClass ns1:Human .

<http://ontology.gaming.network/core#Impression> a owl:Class ;
    rdfs:comment "DEPRECATED legacy IRI. Use 'http://ontology.gaming.network/universal/gaming#Impression' instead."@en ;
    owl:deprecated true ;
    owl:equivalentClass ns1:Impression .

<http://ontology.gaming.network/core#InAppPurchase> a owl:Class ;
    rdfs:comment "DEPRECATED legacy IRI. Use 'http://ontology.gaming.network/universal/gaming#InAppPurchase' instead."@en ;
    owl:deprecated true ;
    owl:equivalentClass ns1:InAppPurchase .

<http://ontology.gaming.network/core#LowEngagement> a owl:Class ;
    rdfs:comment "DEPRECATED legacy IRI. Use 'http://ontology.gaming.network/universal/gaming#LowEngagement' instead."@en ;
    owl:deprecated true ;
    owl:equivalentClass ns1:LowEngagement .

<http://ontology.gaming.network/core#MediumEngagement> a owl:Class ;
    rdfs:comment "DEPRECATED legacy IRI. Use 'http://ontology.gaming.network/universal/gaming#MediumEngagement' instead."@en ;
    owl:deprecated true ;
    owl:equivalentClass ns1:MediumEngagement .

<http://ontology.gaming.network/core#Minnow> a owl:Class ;
    rdfs:comment "DEPRECATED legacy IRI. Use 'http://ontology.gaming.network/universal/gaming#Minnow' instead."@en ;
    owl:deprecated true ;
    owl:equivalentClass ns1:Minnow .

<http://ontology.gaming.network/core#MonetizationSegment> a owl:Class ;
    rdfs:comment "DEPRECATED legacy IRI. Use 'http://ontology.gaming.network/universal/gaming#MonetizationSegment' instead."@en ;
    owl:deprecated true ;
    owl:equivalentClass ns1:MonetizationSegment .

<http://ontology.gaming.network/core#MonetizationThresholds> a owl:Class ;
    rdfs:comment "DEPRECATED legacy IRI. Use 'http://ontology.gaming.network/universal/gaming#MonetizationThresholds' instead."@en ;
    owl:deprecated true ;
    owl:equivalentClass ns1:MonetizationThresholds .

<http://ontology.gaming.network/core#NonPayer> a owl:Class ;
    rdfs:comment "DEPRECATED legacy IRI. Use 'http://ontology.gaming.network/universal/gaming#NonPayer' instead."@en ;
    owl:deprecated true ;
    owl:equivalentClass ns1:NonPayer .

<http://ontology.gaming.network/core#Person> a owl:Class ;
    rdfs:comment "DEPRECATED legacy IRI. Use 'http://ontology.gaming.network/universal/gaming#Person' instead."@en ;
    owl:deprecated true ;
    owl:equivalentClass ns1:Person .

<http://ontology.gaming.network/core#Player> owl:equivalentClass ns1:Player .

<http://ontology.gaming.network/core#Resource> a owl:Class ;
    rdfs:comment "DEPRECATED legacy IRI. Use 'http://ontology.gaming.network/universal/gaming#Resource' instead."@en ;
    owl:deprecated true ;
    owl:equivalentClass ns1:Resource .

<http://ontology.gaming.network/core#Retained> a owl:Class ;
    rdfs:comment "DEPRECATED legacy IRI. Use 'http://ontology.gaming.network/universal/gaming#Retained' instead."@en ;
    owl:deprecated true ;
    owl:equivalentClass ns1:Retained .

<http://ontology.gaming.network/core#RetentionStatus> a owl:Class ;
    rdfs:comment "DEPRECATED legacy IRI. Use 'http://ontology.gaming.network/universal/gaming#RetentionStatus' instead."@en ;
    owl:deprecated true ;
    owl:equivalentClass ns1:RetentionStatus .

<http://ontology.gaming.network/core#Session> a owl:Class ;
    rdfs:comment "DEPRECATED legacy IRI. Use 'http://ontology.gaming.network/universal/human_behavior#Activity' instead."@en ;
    owl:deprecated true ;
    owl:equivalentClass <http://ontology.gaming.network/universal/human_behavior#Activity> .

<http://ontology.gaming.network/core#TestClass> a owl:Class ;
    rdfs:label "Test Class"@en ;
    rdfs:subClassOf <http://ontology.gaming.network/core#Entity> ;
    skos:definition "Test class for E2E testing" .

<http://ontology.gaming.network/core#Transaction> a owl:Class ;
    rdfs:comment "DEPRECATED legacy IRI. Use 'http://ontology.gaming.network/universal/gaming#Transaction' instead."@en ;
    owl:deprecated true ;
    owl:equivalentClass ns1:Transaction .

<http://ontology.gaming.network/core#Whale> a owl:Class ;
    rdfs:comment "DEPRECATED legacy IRI. Use 'http://ontology.gaming.network/universal/gaming#Whale' instead."@en ;
    owl:deprecated true ;
    owl:equivalentClass ns1:Whale .

<http://ontology.gaming.network/core#activityTimestamp> a owl:DatatypeProperty ;
    rdfs:comment "DEPRECATED legacy IRI. Use 'http://ontology.gaming.network/universal/gaming#activityTimestamp' instead."@en ;
    owl:deprecated true ;
    owl:equivalentProperty ns1:activityTimestamp .

<http://ontology.gaming.network/core#advertiserDomain> a owl:DatatypeProperty ;
    rdfs:comment "DEPRECATED legacy IRI. Use 'http://ontology.gaming.network/universal/gaming#advertiserDomain' instead."@en ;
    owl:deprecated true ;
    owl:equivalentProperty ns1:advertiserDomain .

<http://ontology.gaming.network/core#amount> a owl:DatatypeProperty ;
    rdfs:comment "DEPRECATED legacy IRI. Use 'http://ontology.gaming.network/universal/gaming#amount' instead."@en ;
    owl:deprecated true ;
    owl:equivalentProperty ns1:amount .

<http://ontology.gaming.network/core#appliesToTenant> a owl:DatatypeProperty ;
    rdfs:comment "DEPRECATED legacy IRI. Use 'http://ontology.gaming.network/universal/gaming#appliesToTenant' instead."@en ;
    owl:deprecated true ;
    owl:equivalentProperty ns1:appliesToTenant .

<http://ontology.gaming.network/core#attributedTo> a owl:ObjectProperty ;
    rdfs:comment "DEPRECATED legacy IRI. Use 'http://ontology.gaming.network/universal/gaming#attributedTo' instead."@en ;
    owl:deprecated true ;
    owl:equivalentProperty ns1:attributedTo .

<http://ontology.gaming.network/core#belongsToDevice> a owl:ObjectProperty ;
    rdfs:comment "DEPRECATED legacy IRI. Use 'http://ontology.gaming.network/universal/gaming#belongsToDevice' instead."@en ;
    owl:deprecated true ;
    owl:equivalentProperty ns1:belongsToDevice .

<http://ontology.gaming.network/core#belongsToPlayer> owl:equivalentProperty ns1:belongsToPlayer .

<http://ontology.gaming.network/core#bidPrice> a owl:DatatypeProperty ;
    rdfs:comment "DEPRECATED legacy IRI. Use 'http://ontology.gaming.network/universal/gaming#bidPrice' instead."@en ;
    owl:deprecated true ;
    owl:equivalentProperty ns1:bidPrice .

<http://ontology.gaming.network/core#businessDefinition> a owl:AnnotationProperty ;
    rdfs:comment "DEPRECATED legacy IRI. Use 'http://ontology.gaming.network/universal/gaming#businessDefinition' instead."@en ;
    owl:deprecated true ;
    owl:equivalentProperty ns1:businessDefinition .

<http://ontology.gaming.network/core#businessImpact> a owl:AnnotationProperty ;
    rdfs:comment "DEPRECATED legacy IRI. Use 'http://ontology.gaming.network/universal/gaming#businessImpact' instead."@en ;
    owl:deprecated true ;
    owl:equivalentProperty ns1:businessImpact .

<http://ontology.gaming.network/core#businessRationale> a owl:AnnotationProperty ;
    rdfs:comment "DEPRECATED legacy IRI. Use 'http://ontology.gaming.network/universal/gaming#businessRationale' instead."@en ;
    owl:deprecated true ;
    owl:equivalentProperty ns1:businessRationale .

<http://ontology.gaming.network/core#businessTerms> a owl:AnnotationProperty ;
    rdfs:comment "DEPRECATED legacy IRI. Use 'http://ontology.gaming.network/universal/gaming#businessTerms' instead."@en ;
    owl:deprecated true ;
    owl:equivalentProperty ns1:businessTerms .

<http://ontology.gaming.network/core#businessThreshold> a owl:AnnotationProperty ;
    rdfs:comment "DEPRECATED legacy IRI. Use 'http://ontology.gaming.network/universal/gaming#businessThreshold' instead."@en ;
    owl:deprecated true ;
    owl:equivalentProperty ns1:businessThreshold .

<http://ontology.gaming.network/core#businessUseCase> a owl:AnnotationProperty ;
    rdfs:comment "DEPRECATED legacy IRI. Use 'http://ontology.gaming.network/universal/gaming#businessUseCase' instead."@en ;
    owl:deprecated true ;
    owl:equivalentProperty ns1:businessUseCase .

<http://ontology.gaming.network/core#campaignId> a owl:DatatypeProperty,
        owl:FunctionalProperty ;
    rdfs:comment "DEPRECATED legacy IRI. Use 'http://ontology.gaming.network/universal/gaming#campaignId' instead."@en ;
    owl:deprecated true ;
    owl:equivalentProperty ns1:campaignId .

<http://ontology.gaming.network/core#containsBid> a owl:ObjectProperty ;
    rdfs:comment "DEPRECATED legacy IRI. Use 'http://ontology.gaming.network/universal/gaming#containsBid' instead."@en ;
    owl:deprecated true ;
    owl:equivalentProperty ns1:containsBid .

<http://ontology.gaming.network/core#containsEvent> owl:equivalentProperty ns1:containsEvent .

<http://ontology.gaming.network/core#contributedBy> a owl:AnnotationProperty ;
    rdfs:comment "DEPRECATED legacy IRI. Use 'http://ontology.gaming.network/universal/gaming#contributedBy' instead."@en ;
    owl:deprecated true ;
    owl:equivalentProperty ns1:contributedBy .

<http://ontology.gaming.network/core#contributionDate> a owl:AnnotationProperty ;
    rdfs:comment "DEPRECATED legacy IRI. Use 'http://ontology.gaming.network/universal/gaming#contributionDate' instead."@en ;
    owl:deprecated true ;
    owl:equivalentProperty ns1:contributionDate .

<http://ontology.gaming.network/core#country> a owl:DatatypeProperty ;
    rdfs:comment "DEPRECATED legacy IRI. Use 'http://ontology.gaming.network/universal/gaming#country' instead."@en ;
    owl:deprecated true ;
    owl:equivalentProperty ns1:country .

<http://ontology.gaming.network/core#currency> a owl:DatatypeProperty ;
    rdfs:comment "DEPRECATED legacy IRI. Use 'http://ontology.gaming.network/universal/gaming#currency' instead."@en ;
    owl:deprecated true ;
    owl:equivalentProperty ns1:currency .

<http://ontology.gaming.network/core#deviceId> a owl:DatatypeProperty,
        owl:FunctionalProperty ;
    rdfs:comment "DEPRECATED legacy IRI. Use 'http://ontology.gaming.network/universal/gaming#deviceId' instead."@en ;
    owl:deprecated true ;
    owl:equivalentProperty ns1:deviceId .

<http://ontology.gaming.network/core#deviceOS> a owl:DatatypeProperty ;
    rdfs:comment "DEPRECATED legacy IRI. Use 'http://ontology.gaming.network/universal/gaming#deviceOS' instead."@en ;
    owl:deprecated true ;
    owl:equivalentProperty ns1:deviceOS .

<http://ontology.gaming.network/core#deviceType> a owl:DatatypeProperty ;
    rdfs:comment "DEPRECATED legacy IRI. Use 'http://ontology.gaming.network/universal/gaming#deviceType' instead."@en ;
    owl:deprecated true ;
    owl:equivalentProperty ns1:deviceType .

<http://ontology.gaming.network/core#dolphinIapThreshold> a owl:DatatypeProperty ;
    rdfs:comment "DEPRECATED legacy IRI. Use 'http://ontology.gaming.network/universal/gaming#dolphinIapThreshold' instead."@en ;
    owl:deprecated true ;
    owl:equivalentProperty ns1:dolphinIapThreshold .

<http://ontology.gaming.network/core#dolphinMonetaryThreshold> a owl:DatatypeProperty ;
    rdfs:comment "DEPRECATED legacy IRI. Use 'http://ontology.gaming.network/universal/gaming#dolphinMonetaryThreshold' instead."@en ;
    owl:deprecated true ;
    owl:equivalentProperty ns1:dolphinMonetaryThreshold .

<http://ontology.gaming.network/core#eventType> a owl:DatatypeProperty ;
    rdfs:comment "DEPRECATED legacy IRI. Use 'http://ontology.gaming.network/universal/gaming#eventType' instead."@en ;
    owl:deprecated true ;
    owl:equivalentProperty ns1:eventType .

<http://ontology.gaming.network/core#hasAdInteraction> a owl:ObjectProperty ;
    rdfs:comment "DEPRECATED legacy IRI. Use 'http://ontology.gaming.network/universal/gaming#hasAdInteraction' instead."@en ;
    owl:deprecated true ;
    owl:equivalentProperty ns1:hasAdInteraction .

<http://ontology.gaming.network/core#hasAttributedInstall> a owl:ObjectProperty ;
    rdfs:comment "DEPRECATED legacy IRI. Use 'http://ontology.gaming.network/universal/gaming#hasAttributedInstall' instead."@en ;
    owl:deprecated true ;
    owl:equivalentProperty ns1:hasAttributedInstall .

<http://ontology.gaming.network/core#hasEngagementLevel> a owl:ObjectProperty ;
    rdfs:comment "DEPRECATED legacy IRI. Use 'http://ontology.gaming.network/universal/gaming#hasEngagementLevel' instead."@en ;
    owl:deprecated true ;
    owl:equivalentProperty ns1:hasEngagementLevel .

<http://ontology.gaming.network/core#hasImpression> a owl:ObjectProperty ;
    rdfs:comment "DEPRECATED legacy IRI. Use 'http://ontology.gaming.network/universal/gaming#hasImpression' instead."@en ;
    owl:deprecated true ;
    owl:equivalentProperty ns1:hasImpression .

<http://ontology.gaming.network/core#hasInAppPurchase> a owl:ObjectProperty ;
    rdfs:comment "DEPRECATED legacy IRI. Use 'http://ontology.gaming.network/universal/gaming#hasInAppPurchase' instead."@en ;
    owl:deprecated true ;
    owl:equivalentProperty ns1:hasInAppPurchase .

<http://ontology.gaming.network/core#hasMonetizationSegment> a owl:ObjectProperty ;
    rdfs:comment "DEPRECATED legacy IRI. Use 'http://ontology.gaming.network/universal/gaming#hasMonetizationSegment' instead."@en ;
    owl:deprecated true ;
    owl:equivalentProperty ns1:hasMonetizationSegment .

<http://ontology.gaming.network/core#hasRetentionStatus> a owl:ObjectProperty ;
    rdfs:comment "DEPRECATED legacy IRI. Use 'http://ontology.gaming.network/universal/gaming#hasRetentionStatus' instead."@en ;
    owl:deprecated true ;
    owl:equivalentProperty ns1:hasRetentionStatus .

<http://ontology.gaming.network/core#hasSession> a owl:ObjectProperty ;
    rdfs:comment "DEPRECATED legacy IRI. Use 'http://ontology.gaming.network/universal/gaming#hasSession' instead."@en ;
    owl:deprecated true ;
    owl:equivalentProperty ns1:hasSession .

<http://ontology.gaming.network/core#lastReviewed> a owl:AnnotationProperty ;
    rdfs:comment "DEPRECATED legacy IRI. Use 'http://ontology.gaming.network/universal/gaming#lastReviewed' instead."@en ;
    owl:deprecated true ;
    owl:equivalentProperty ns1:lastReviewed .

<http://ontology.gaming.network/core#minnowIapThreshold> a owl:DatatypeProperty ;
    rdfs:comment "DEPRECATED legacy IRI. Use 'http://ontology.gaming.network/universal/gaming#minnowIapThreshold' instead."@en ;
    owl:deprecated true ;
    owl:equivalentProperty ns1:minnowIapThreshold .

<http://ontology.gaming.network/core#minnowMonetaryThreshold> a owl:DatatypeProperty ;
    rdfs:comment "DEPRECATED legacy IRI. Use 'http://ontology.gaming.network/universal/gaming#minnowMonetaryThreshold' instead."@en ;
    owl:deprecated true ;
    owl:equivalentProperty ns1:minnowMonetaryThreshold .

<http://ontology.gaming.network/core#occursInGame> a owl:ObjectProperty ;
    rdfs:comment "DEPRECATED legacy IRI. Use 'http://ontology.gaming.network/universal/gaming#occursInGame' instead."@en ;
    owl:deprecated true ;
    owl:equivalentProperty ns1:occursInGame .

<http://ontology.gaming.network/core#occursInSession> owl:equivalentProperty ns1:occursInSession .

<http://ontology.gaming.network/core#partOfCampaign> a owl:ObjectProperty ;
    rdfs:comment "DEPRECATED legacy IRI. Use 'http://ontology.gaming.network/universal/gaming#partOfCampaign' instead."@en ;
    owl:deprecated true ;
    owl:equivalentProperty ns1:partOfCampaign .

<http://ontology.gaming.network/core#playsGame> a owl:ObjectProperty ;
    rdfs:comment "DEPRECATED legacy IRI. Use 'http://ontology.gaming.network/universal/gaming#playsGame' instead."@en ;
    owl:deprecated true ;
    owl:equivalentProperty ns1:playsGame .

<http://ontology.gaming.network/core#sessionCount> a owl:DatatypeProperty ;
    rdfs:comment "DEPRECATED legacy IRI. Use 'http://ontology.gaming.network/universal/gaming#sessionCount' instead."@en ;
    owl:deprecated true ;
    owl:equivalentProperty ns1:sessionCount .

<http://ontology.gaming.network/core#sessionDuration> owl:equivalentProperty ns1:sessionDuration .

<http://ontology.gaming.network/core#sessionId> a owl:DatatypeProperty,
        owl:FunctionalProperty ;
    rdfs:comment "DEPRECATED legacy IRI. Use 'http://ontology.gaming.network/universal/gaming#sessionId' instead."@en ;
    owl:deprecated true ;
    owl:equivalentProperty ns1:sessionId .

<http://ontology.gaming.network/core#totalSpent> a owl:DatatypeProperty ;
    rdfs:comment "DEPRECATED legacy IRI. Use 'http://ontology.gaming.network/universal/gaming#totalSpent' instead."@en ;
    owl:deprecated true ;
    owl:equivalentProperty ns1:totalSpent .

<http://ontology.gaming.network/core#whaleIapThreshold> a owl:DatatypeProperty ;
    rdfs:comment "DEPRECATED legacy IRI. Use 'http://ontology.gaming.network/universal/gaming#whaleIapThreshold' instead."@en ;
    owl:deprecated true ;
    owl:equivalentProperty ns1:whaleIapThreshold .

<http://ontology.gaming.network/core#whaleMonetaryThreshold> a owl:DatatypeProperty ;
    rdfs:comment "DEPRECATED legacy IRI. Use 'http://ontology.gaming.network/universal/gaming#whaleMonetaryThreshold' instead."@en ;
    owl:deprecated true ;
    owl:equivalentProperty ns1:whaleMonetaryThreshold .

<http://ontology.gaming.network/universal/bridge> a owl:Ontology ;
    rdfs:comment "Alignment axioms mapping core gaming ontology terms to universal foundations." .

ns1:AdViewed a owl:Class ;
    rdfs:label "Ad Viewed"@en ;
    rdfs:subClassOf ns1:MonetizationEvent ;
    skos:definition "Advertisement impression event" .

ns1:GameEnd a owl:Class ;
    rdfs:label "Game End"@en ;
    rdfs:subClassOf ns1:EngagementEvent ;
    skos:definition "Game completion event" .

ns1:GameStart a owl:Class ;
    rdfs:label "Game Start"@en ;
    rdfs:subClassOf ns1:EngagementEvent ;
    skos:definition "Game initialization event" .

ns1:LevelComplete a owl:Class ;
    rdfs:label "Level Complete"@en ;
    rdfs:subClassOf ns1:EngagementEvent ;
    skos:definition "Level completion event" .

ns1:LevelFail a owl:Class ;
    rdfs:label "Level Fail"@en ;
    rdfs:subClassOf ns1:EngagementEvent ;
    skos:definition "Level failure event" .

ns1:LevelStart a owl:Class ;
    rdfs:label "Level Start"@en ;
    rdfs:subClassOf ns1:EngagementEvent ;
    skos:definition "Level initialization event" .

ns1:ProgressionEvent a owl:Class ;
    rdfs:label "Progression Event"@en ;
    rdfs:comment "Events related to player progression." ;
    rdfs:subClassOf ns1:GameEvent ;
    skos:definition "Progression events (LevelUp, SkillUnlock, Milestone)" .

ns1:Purchase a owl:Class ;
    rdfs:label "Purchase"@en ;
    rdfs:subClassOf ns1:MonetizationEvent ;
    skos:definition "Purchase event (in-app purchase, subscription)" .

ns1:SocialEvent a owl:Class ;
    rdfs:label "Social Event"@en ;
    rdfs:comment "Events related to social interactions in games." ;
    rdfs:subClassOf ns1:GameEvent ;
    skos:definition "Social events (MultiplayerJoin, FriendInvite, ChatMessage)" .

ns1:difficulty a owl:DatatypeProperty ;
    rdfs:label "difficulty"@en ;
    rdfs:domain ns1:EngagementEvent ;
    rdfs:range xsd:string ;
    skos:definition "Difficulty level (easy, medium, hard)" .

ns1:engagementScore a owl:DatatypeProperty ;
    rdfs:label "engagement score"@en ;
    rdfs:domain ns1:Player ;
    rdfs:range xsd:decimal ;
    skos:definition "Calculated engagement metric" .

ns1:gameGenre a owl:DatatypeProperty ;
    rdfs:label "game genre"@en ;
    rdfs:domain ns1:Game ;
    rdfs:range xsd:string ;
    skos:definition "Genre of the game (Action, RPG, Puzzle, etc.)" .

ns1:gameId a owl:DatatypeProperty,
        owl:FunctionalProperty ;
    rdfs:label "game ID"@en ;
    rdfs:domain ns1:Game ;
    rdfs:range xsd:string ;
    skos:definition "Unique identifier for a game" .

ns1:gameName a owl:DatatypeProperty ;
    rdfs:label "game name"@en ;
    rdfs:domain ns1:Game ;
    rdfs:range xsd:string ;
    skos:definition "Name of the game" .

ns1:hasPlayerState a owl:ObjectProperty ;
    rdfs:label "has player state"@en ;
    rdfs:domain ns1:Player ;
    rdfs:range ns1:PlayerState ;
    skos:definition "Relates a player to their current state" .

ns1:itemId a owl:DatatypeProperty ;
    rdfs:label "item ID"@en ;
    rdfs:domain ns1:MonetizationEvent ;
    rdfs:range xsd:string ;
    skos:definition "Item/product identifier" .

ns1:levelNumber a owl:DatatypeProperty ;
    rdfs:label "level number"@en ;
    rdfs:domain ns1:EngagementEvent ;
    rdfs:range xsd:integer ;
    skos:definition "Level identifier/number" .

ns1:retentionDay a owl:DatatypeProperty ;
    rdfs:label "retention day"@en ;
    rdfs:domain ns1:Player ;
    rdfs:range xsd:integer ;
    skos:definition "Day X retention status (1, 7, 30)" .

ns1:similarBehaviorTo a owl:ObjectProperty,
        owl:SymmetricProperty ;
    rdfs:label "similar behavior to"@en ;
    rdfs:domain ns1:Player ;
    rdfs:range ns1:Player ;
    skos:definition "Relates players with similar behavioral patterns (across games)" .

ns1:similarEventTypeTo a owl:ObjectProperty,
        owl:SymmetricProperty ;
    rdfs:label "similar event type to"@en ;
    rdfs:domain ns1:GameEvent ;
    rdfs:range ns1:GameEvent ;
    skos:definition "Relates similar event types across games" .

ns1:similarGenreTo a owl:ObjectProperty,
        owl:SymmetricProperty ;
    rdfs:label "similar genre to"@en ;
    rdfs:domain ns1:Game ;
    rdfs:range ns1:Game ;
    skos:definition "Relates games with similar genres" .

ns1:totalIaps a owl:DatatypeProperty ;
    rdfs:label "total IAPs"@en ;
    rdfs:domain ns1:Player ;
    rdfs:range xsd:integer ;
    skos:definition "Total in-app purchases for this player" .

<http://ontology.gaming.network/universal/gaming_ontology> a owl:Ontology ;
    dc:creator "WorldModelData" ;
    dc:title "WorldModelData Universal Gaming Ontology v1"@en ;
    rdfs:comment "Flagship universal gaming ontology release. Flattened distribution containing the universal foundations plus absorbed legacy core semantics."@en ;
    owl:imports <http://ontology.gaming.network/universal/gaming>,
        <http://ontology.gaming.network/universal/human_behavior> ;
    owl:versionInfo "1.0.0" .

<http://ontology.gaming.network/universal/human_behavior#activityDuration> a owl:DatatypeProperty ;
    rdfs:label "activity duration"@en ;
    rdfs:comment "Universal temporal property for activity duration." ;
    rdfs:domain <http://ontology.gaming.network/universal/human_behavior#Activity> ;
    rdfs:range xsd:integer ;
    skos:definition "Duration of the activity in seconds" .

<http://ontology.gaming.network/universal/human_behavior#activityEndTimestamp> a owl:DatatypeProperty ;
    rdfs:label "activity end timestamp"@en ;
    rdfs:comment "Universal temporal property for activity end time." ;
    rdfs:domain <http://ontology.gaming.network/universal/human_behavior#Activity> ;
    rdfs:range xsd:dateTime ;
    skos:definition "Timestamp when the activity ended" .

<http://ontology.gaming.network/universal/human_behavior#activityId> a owl:DatatypeProperty,
        owl:FunctionalProperty ;
    rdfs:label "activity ID"@en ;
    rdfs:comment "Universal identifier property for any activity type." ;
    rdfs:domain <http://ontology.gaming.network/universal/human_behavior#Activity> ;
    rdfs:range xsd:string ;
    skos:definition "Unique identifier for an activity" .

<http://ontology.gaming.network/universal/human_behavior#activityStartTimestamp> a owl:DatatypeProperty ;
    rdfs:label "activity start timestamp"@en ;
    rdfs:comment "Universal temporal property for activity start time." ;
    rdfs:domain <http://ontology.gaming.network/universal/human_behavior#Activity> ;
    rdfs:range xsd:dateTime ;
    skos:definition "Timestamp when the activity started" .

<http://ontology.gaming.network/universal/human_behavior#activityTimestamp> a owl:DatatypeProperty ;
    rdfs:label "activity timestamp"@en ;
    rdfs:comment "Universal temporal property for any behavioral event type." ;
    rdfs:domain <http://ontology.gaming.network/universal/human_behavior#BehavioralEvent> ;
    rdfs:range xsd:dateTime ;
    skos:definition "Timestamp when the behavioral event occurred" .

<http://ontology.gaming.network/universal/human_behavior#actorId> a owl:DatatypeProperty,
        owl:FunctionalProperty ;
    rdfs:label "actor ID"@en ;
    rdfs:comment "Universal identifier property for any human actor type." ;
    rdfs:domain <http://ontology.gaming.network/universal/human_behavior#HumanActor> ;
    rdfs:range xsd:string ;
    skos:definition "Unique identifier for a human actor" .

<http://ontology.gaming.network/universal/human_behavior#eventId> a owl:DatatypeProperty,
        owl:FunctionalProperty ;
    rdfs:label "event ID"@en ;
    rdfs:comment "Universal identifier property for any behavioral event type." ;
    rdfs:domain <http://ontology.gaming.network/universal/human_behavior#BehavioralEvent> ;
    rdfs:range xsd:string ;
    skos:definition "Unique identifier for a behavioral event" .

<http://ontology.gaming.network/universal/human_behavior#generatesEvent> a owl:ObjectProperty ;
    rdfs:label "generates event"@en ;
    rdfs:domain <http://ontology.gaming.network/universal/human_behavior#Activity> ;
    rdfs:range <http://ontology.gaming.network/universal/human_behavior#BehavioralEvent> ;
    owl:inverseOf <http://ontology.gaming.network/universal/human_behavior#generatedByActivity> ;
    skos:definition "Relates an activity to behavioral events it generates" .

<http://ontology.gaming.network/universal/human_behavior#hasEngagementLevel> a owl:ObjectProperty ;
    rdfs:label "has engagement level"@en ;
    rdfs:comment "Universal property for engagement classification across domains." ;
    rdfs:domain <http://ontology.gaming.network/universal/human_behavior#HumanActor> ;
    rdfs:range <http://ontology.gaming.network/universal/human_behavior#BehavioralState> ;
    skos:definition "Applies to gaming (player engagement), treatment (patient engagement), task performance (user engagement)" .

<http://ontology.gaming.network/universal/human_behavior#hasRetentionStatus> a owl:ObjectProperty ;
    rdfs:label "has retention status"@en ;
    rdfs:comment "Universal property for retention classification across domains." ;
    rdfs:domain <http://ontology.gaming.network/universal/human_behavior#HumanActor> ;
    rdfs:range <http://ontology.gaming.network/universal/human_behavior#BehavioralState> ;
    skos:definition "Applies to player retention (gaming), treatment adherence (healthcare), customer retention (finance)" .

<http://ontology.gaming.network/universal/human_behavior#hasSocialContext> a owl:ObjectProperty ;
    rdfs:label "has social context"@en ;
    rdfs:comment "Universal property for social context across domains." ;
    rdfs:domain <http://ontology.gaming.network/universal/human_behavior#HumanActor> ;
    rdfs:range <http://ontology.gaming.network/universal/human_behavior#BehavioralState> ;
    skos:definition "Applies to multiplayer games (gaming), social support (healthcare), network effects (finance)" .

<http://ontology.gaming.network/universal/human_behavior#hasState> a owl:ObjectProperty ;
    rdfs:label "has state"@en ;
    rdfs:domain <http://ontology.gaming.network/universal/human_behavior#HumanActor> ;
    rdfs:range <http://ontology.gaming.network/universal/human_behavior#BehavioralState> ;
    owl:inverseOf <http://ontology.gaming.network/universal/human_behavior#stateOfActor> ;
    skos:definition "Relates a human actor to their behavioral state" .

<http://ontology.gaming.network/universal/human_behavior#hasTemporalPattern> a owl:ObjectProperty ;
    rdfs:label "has temporal pattern"@en ;
    rdfs:comment "Universal property for temporal behavior patterns across domains." ;
    rdfs:domain <http://ontology.gaming.network/universal/human_behavior#HumanActor> ;
    rdfs:range <http://ontology.gaming.network/universal/human_behavior#BehavioralState> ;
    skos:definition "Applies to session frequency (gaming), treatment frequency (healthcare), activity frequency (finance)" .

<http://ontology.gaming.network/universal/human_behavior#hasValueSegment> a owl:ObjectProperty ;
    rdfs:label "has value segment"@en ;
    rdfs:comment "Universal property for value segmentation across domains." ;
    rdfs:domain <http://ontology.gaming.network/universal/human_behavior#HumanActor> ;
    rdfs:range <http://ontology.gaming.network/universal/human_behavior#BehavioralState> ;
    skos:definition "Applies to monetization (gaming), treatment compliance (healthcare), customer value (finance)" .

<http://ontology.gaming.network/universal/human_behavior#influencesState> a owl:ObjectProperty ;
    rdfs:label "influences state"@en ;
    rdfs:domain <http://ontology.gaming.network/universal/human_behavior#BehavioralEvent> ;
    rdfs:range <http://ontology.gaming.network/universal/human_behavior#BehavioralState> ;
    owl:inverseOf <http://ontology.gaming.network/universal/human_behavior#influencedByEvent> ;
    skos:definition "Relates a behavioral event to behavioral states it influences" .

<http://ontology.gaming.network/universal/human_behavior#performsActivity> a owl:ObjectProperty ;
    rdfs:label "performs activity"@en ;
    rdfs:domain <http://ontology.gaming.network/universal/human_behavior#HumanActor> ;
    rdfs:range <http://ontology.gaming.network/universal/human_behavior#Activity> ;
    owl:inverseOf <http://ontology.gaming.network/universal/human_behavior#performedByActor> ;
    skos:definition "Relates a human actor to activities they perform" .

<http://ontology.gaming.network/universal/human_behavior#similarTo> a owl:ObjectProperty,
        owl:SymmetricProperty ;
    rdfs:label "similar to"@en ;
    rdfs:comment "Used for behavioral similarity analysis and pattern recognition." ;
    rdfs:domain <http://ontology.gaming.network/universal/human_behavior#HumanActor> ;
    rdfs:range <http://ontology.gaming.network/universal/human_behavior#HumanActor> ;
    skos:definition "Relates human actors with similar behavioral patterns" .

<http://ontology.gaming.network/core#Entity> a owl:Class ;
    rdfs:comment "DEPRECATED legacy IRI. Use 'http://ontology.gaming.network/universal/gaming#Entity' instead."@en ;
    owl:deprecated true ;
    owl:equivalentClass ns1:Entity .

<http://ontology.gaming.network/universal/gaming> a owl:Ontology ;
    dc:creator "Gi Fernando" ;
    dc:date "2025-12-27" ;
    dc:title "Universal Gaming Foundation Ontology v1.0" ;
    rdfs:comment "Comprehensive gaming ontology extending universal human behavior foundation" ;
    owl:imports <http://ontology.gaming.network/universal/human_behavior> ;
    owl:versionInfo "1.0.0" .

ns1:Human a owl:Class ;
    rdfs:label "New Class"@en ;
    rdfs:subClassOf ns1:Person ;
    skos:definition "A Human being" .

ns1:Resource a owl:Class ;
    rdfs:label "Resource"@en ;
    rdfs:subClassOf ns1:Entity ;
    skos:definition "A resource used or consumed in the gaming ecosystem" .

ns1:activityTimestamp a owl:DatatypeProperty ;
    rdfs:label "activity timestamp"@en ;
    rdfs:domain <http://ontology.gaming.network/universal/human_behavior#BehavioralEvent> ;
    rdfs:range xsd:dateTime ;
    skos:definition "Timestamp when the event occurred" .

ns1:advertiserDomain a owl:DatatypeProperty ;
    rdfs:label "advertiser domain"@en ;
    rdfs:domain ns1:Campaign ;
    rdfs:range xsd:string ;
    skos:definition "Domain of the advertiser" .

ns1:amount a owl:DatatypeProperty ;
    rdfs:label "amount"@en ;
    rdfs:domain ns1:MonetizationEvent,
        ns1:Transaction ;
    rdfs:range xsd:decimal ;
    skos:definition "Transaction amount" .

ns1:appliesToTenant a owl:DatatypeProperty ;
    rdfs:label "applies to tenant"@en ;
    rdfs:domain ns1:MonetizationThresholds ;
    rdfs:range xsd:string ;
    skos:definition "Tenant identifier this threshold configuration applies to"@en .

ns1:attributedTo a owl:ObjectProperty ;
    rdfs:label "attributed to"@en ;
    rdfs:domain ns1:AttributedInstall ;
    rdfs:range ns1:Campaign ;
    skos:definition "Relates an install to the campaign that drove it" .

ns1:bidPrice a owl:DatatypeProperty ;
    rdfs:label "bid price"@en ;
    rdfs:domain ns1:Bid ;
    rdfs:range xsd:decimal ;
    skos:definition "Price of the bid in the ad auction" .

ns1:businessDefinition a owl:AnnotationProperty ;
    rdfs:label "business definition"@en ;
    rdfs:comment "Plain-language business definition of a concept (multi-language supported via language tags)."@en .

ns1:businessImpact a owl:AnnotationProperty ;
    rdfs:label "business impact"@en ;
    rdfs:comment "Business value/impact statement for the concept (e.g., HIGH/MEDIUM/LOW with rationale)."@en .

ns1:businessRationale a owl:AnnotationProperty ;
    rdfs:label "business rationale"@en ;
    rdfs:comment "Why this concept matters from a business perspective (multi-language supported via language tags)."@en .

ns1:businessTerms a owl:AnnotationProperty ;
    rdfs:label "business terms"@en ;
    rdfs:comment "Business terminology/synonyms used for the concept (multi-language supported via language tags)."@en .

ns1:businessThreshold a owl:AnnotationProperty ;
    rdfs:label "business threshold"@en ;
    rdfs:comment "Business thresholds/criteria used to operationalize the concept (multi-language supported via language tags)."@en .

ns1:businessUseCase a owl:AnnotationProperty ;
    rdfs:label "business use case"@en ;
    rdfs:comment "Real-world business use cases for the concept (multi-language supported via language tags)."@en .

ns1:campaignId a owl:DatatypeProperty,
        owl:FunctionalProperty ;
    rdfs:label "campaign ID"@en ;
    rdfs:domain ns1:Campaign ;
    rdfs:range xsd:string ;
    skos:definition "Unique identifier for a campaign" .

ns1:containsBid a owl:ObjectProperty ;
    rdfs:label "contains bid"@en ;
    rdfs:domain <http://ontology.gaming.network/universal/human_behavior#Activity> ;
    rdfs:range ns1:Bid ;
    skos:definition "Relates a session to bids that occurred during it" .

ns1:containsEvent a owl:ObjectProperty ;
    rdfs:label "contains event"@en ;
    rdfs:domain ns1:GameSession ;
    rdfs:range ns1:GameEvent ;
    owl:inverseOf ns1:occursInSession ;
    skos:definition "Relates a gaming session to events it contains" .

ns1:contributedBy a owl:AnnotationProperty ;
    rdfs:label "contributed by"@en ;
    rdfs:comment "Provenance: identifier of the contributor (domain expert, ontology editor, etc.)."@en .

ns1:contributionDate a owl:AnnotationProperty ;
    rdfs:label "contribution date"@en ;
    rdfs:comment "Provenance: date of contribution (xsd:date)."@en .

ns1:country a owl:DatatypeProperty ;
    rdfs:label "country"@en ;
    rdfs:domain ns1:Player ;
    rdfs:range xsd:string ;
    skos:definition "Country code of the device" .

ns1:currency a owl:DatatypeProperty ;
    rdfs:label "currency"@en ;
    rdfs:domain ns1:MonetizationEvent,
        ns1:Transaction ;
    rdfs:range xsd:string ;
    skos:definition "Currency code",
        "Currency code for the transaction" .

ns1:deviceId a owl:DatatypeProperty,
        owl:FunctionalProperty ;
    rdfs:label "device ID"@en ;
    rdfs:comment "Maps to ub:actorId in universal foundation." ;
    rdfs:domain ns1:Player ;
    rdfs:range xsd:string ;
    skos:definition "Unique identifier for a device",
        "Unique identifier for a player/device" .

ns1:deviceOS a owl:DatatypeProperty ;
    rdfs:label "device OS"@en ;
    rdfs:domain ns1:Player ;
    rdfs:range xsd:string ;
    skos:definition "Operating system of the device" .

ns1:deviceType a owl:DatatypeProperty ;
    rdfs:label "device type"@en ;
    rdfs:domain ns1:Player ;
    rdfs:range xsd:string ;
    skos:definition "Type of device (phone, tablet, etc.)" .

ns1:dolphinIapThreshold a owl:DatatypeProperty ;
    rdfs:label "dolphin IAP threshold"@en ;
    rdfs:domain ns1:MonetizationThresholds ;
    rdfs:range xsd:integer ;
    skos:definition "Minimum IAP count to classify as Dolphin"@en .

ns1:dolphinMonetaryThreshold a owl:DatatypeProperty ;
    rdfs:label "dolphin monetary threshold"@en ;
    rdfs:domain ns1:MonetizationThresholds ;
    rdfs:range xsd:decimal ;
    skos:definition "Minimum monetary value (£) to classify as Dolphin (future use)"@en .

ns1:eventType a owl:DatatypeProperty ;
    rdfs:label "event type"@en ;
    rdfs:domain ns1:GameEvent,
        <http://ontology.gaming.network/universal/human_behavior#BehavioralEvent> ;
    rdfs:range xsd:string ;
    skos:definition "Type of event",
        "Type of gaming event" .

ns1:hasAdInteraction a owl:ObjectProperty ;
    rdfs:label "has ad interaction"@en ;
    rdfs:domain <http://ontology.gaming.network/universal/human_behavior#Activity> ;
    rdfs:range ns1:AdInteraction ;
    skos:definition "Relates a session to ad interactions during it" .

ns1:hasAttributedInstall a owl:ObjectProperty ;
    rdfs:label "has attributed install"@en ;
    rdfs:domain ns1:Player ;
    rdfs:range ns1:AttributedInstall ;
    skos:definition "Relates a device to its attributed install event" .

ns1:hasEngagementLevel a owl:ObjectProperty ;
    rdfs:label "has engagement level"@en ;
    rdfs:domain ns1:Player ;
    rdfs:range ns1:EngagementLevel ;
    skos:definition "Relates a device to its inferred engagement classification",
        "Relates a player to their engagement level classification" .

ns1:hasImpression a owl:ObjectProperty ;
    rdfs:label "has impression"@en ;
    rdfs:domain <http://ontology.gaming.network/universal/human_behavior#Activity> ;
    rdfs:range ns1:Impression ;
    skos:definition "Relates a session to ad impressions shown during it" .

ns1:hasInAppPurchase a owl:ObjectProperty ;
    rdfs:label "has in-app purchase"@en ;
    rdfs:domain <http://ontology.gaming.network/universal/human_behavior#Activity> ;
    rdfs:range ns1:InAppPurchase ;
    skos:definition "Relates a session to purchases made during it" .

ns1:hasMonetizationSegment a owl:ObjectProperty ;
    rdfs:label "has monetization segment"@en ;
    rdfs:domain ns1:Player ;
    rdfs:range ns1:MonetizationSegment ;
    skos:definition "Relates a device to its inferred monetization classification",
        "Relates a player to their monetization segment classification" .

ns1:hasRetentionStatus a owl:ObjectProperty ;
    rdfs:label "has retention status"@en ;
    rdfs:domain ns1:Player ;
    rdfs:range ns1:RetentionStatus ;
    skos:definition "Relates a device to its inferred retention status",
        "Relates a player to their retention status classification" .

ns1:hasSession a owl:ObjectProperty ;
    rdfs:label "has session"@en ;
    rdfs:domain ns1:Player ;
    rdfs:range ns1:GameSession,
        <http://ontology.gaming.network/universal/human_behavior#Activity> ;
    owl:inverseOf ns1:belongsToDevice,
        ns1:belongsToPlayer ;
    skos:definition "Relates a device to its sessions",
        "Relates a player to their gaming sessions" .

ns1:lastReviewed a owl:AnnotationProperty ;
    rdfs:label "last reviewed"@en ;
    rdfs:comment "Provenance: date this business semantics annotation was last reviewed (xsd:date)."@en .

ns1:minnowIapThreshold a owl:DatatypeProperty ;
    rdfs:label "minnow IAP threshold"@en ;
    rdfs:domain ns1:MonetizationThresholds ;
    rdfs:range xsd:integer ;
    skos:definition "Minimum IAP count to classify as Minnow"@en .

ns1:minnowMonetaryThreshold a owl:DatatypeProperty ;
    rdfs:label "minnow monetary threshold"@en ;
    rdfs:domain ns1:MonetizationThresholds ;
    rdfs:range xsd:decimal ;
    skos:definition "Minimum monetary value (£) to classify as Minnow (future use)"@en .

ns1:occursInGame a owl:ObjectProperty ;
    rdfs:label "occurs in game"@en ;
    rdfs:domain ns1:GameSession,
        <http://ontology.gaming.network/universal/human_behavior#Activity> ;
    rdfs:range ns1:Game ;
    skos:definition "Relates a gaming session to the game it occurs in",
        "Relates a session to the game it occurs in" .

ns1:partOfCampaign a owl:ObjectProperty ;
    rdfs:label "part of campaign"@en ;
    rdfs:domain ns1:AdEvent ;
    rdfs:range ns1:Campaign ;
    skos:definition "Relates an ad event to its campaign" .

ns1:playsGame a owl:ObjectProperty ;
    rdfs:label "plays game"@en ;
    rdfs:comment "Inferred from hasSession and occursInGame" ;
    rdfs:domain ns1:Player ;
    rdfs:range ns1:Game ;
    skos:definition "Relates a device to games it plays",
        "Relates a player to games they play" .

ns1:sessionCount a owl:DatatypeProperty ;
    rdfs:label "session count"@en ;
    rdfs:domain ns1:Player ;
    rdfs:range xsd:integer ;
    skos:definition "Number of gaming sessions for this player",
        "Total number of sessions for this device" .

ns1:sessionDuration a owl:DatatypeProperty ;
    rdfs:label "session duration"@en ;
    rdfs:comment "Maps to ub:activityDuration in universal foundation." ;
    rdfs:domain ns1:GameSession ;
    rdfs:range xsd:integer ;
    skos:definition "Duration of gaming session in seconds" .

ns1:sessionId a owl:DatatypeProperty,
        owl:FunctionalProperty ;
    rdfs:label "session ID"@en ;
    rdfs:comment "Maps to ub:activityId in universal foundation." ;
    rdfs:domain ns1:GameSession,
        <http://ontology.gaming.network/universal/human_behavior#Activity> ;
    rdfs:range xsd:string ;
    skos:definition "Unique identifier for a gaming session",
        "Unique identifier for a session" .

ns1:totalSpent a owl:DatatypeProperty ;
    rdfs:label "total spent"@en ;
    rdfs:domain ns1:Player ;
    rdfs:range xsd:decimal ;
    skos:definition "Total amount spent by this device" .

ns1:whaleIapThreshold a owl:DatatypeProperty ;
    rdfs:label "whale IAP threshold"@en ;
    rdfs:domain ns1:MonetizationThresholds ;
    rdfs:range xsd:integer ;
    skos:definition "Minimum IAP count to classify as Whale"@en .

ns1:whaleMonetaryThreshold a owl:DatatypeProperty ;
    rdfs:label "whale monetary threshold"@en ;
    rdfs:domain ns1:MonetizationThresholds ;
    rdfs:range xsd:decimal ;
    skos:definition "Minimum monetary value (£) to classify as Whale (future use)"@en .

<http://ontology.gaming.network/universal/human_behavior#generatedByActivity> a owl:ObjectProperty ;
    rdfs:label "generated by activity"@en ;
    rdfs:domain <http://ontology.gaming.network/universal/human_behavior#BehavioralEvent> ;
    rdfs:range <http://ontology.gaming.network/universal/human_behavior#Activity> ;
    skos:definition "Relates a behavioral event to the activity that generated it" .

<http://ontology.gaming.network/universal/human_behavior#influencedByEvent> a owl:ObjectProperty ;
    rdfs:label "influenced by event"@en ;
    rdfs:domain <http://ontology.gaming.network/universal/human_behavior#BehavioralState> ;
    rdfs:range <http://ontology.gaming.network/universal/human_behavior#BehavioralEvent> ;
    skos:definition "Relates a behavioral state to events that influence it" .

<http://ontology.gaming.network/universal/human_behavior#performedByActor> a owl:ObjectProperty ;
    rdfs:label "performed by actor"@en ;
    rdfs:domain <http://ontology.gaming.network/universal/human_behavior#Activity> ;
    rdfs:range <http://ontology.gaming.network/universal/human_behavior#HumanActor> ;
    skos:definition "Relates an activity to the human actor performing it" .

<http://ontology.gaming.network/universal/human_behavior#stateOfActor> a owl:ObjectProperty ;
    rdfs:label "state of actor"@en ;
    rdfs:domain <http://ontology.gaming.network/universal/human_behavior#BehavioralState> ;
    rdfs:range <http://ontology.gaming.network/universal/human_behavior#HumanActor> ;
    skos:definition "Relates a behavioral state to the human actor it describes" .

ns1:ActivePlayer a owl:Class ;
    rdfs:label "Active Player"@en ;
    rdfs:subClassOf ns1:PlayerState ;
    skos:definition "Currently active player" .

ns1:AdInteraction a owl:Class ;
    rdfs:label "Ad Interaction"@en ;
    rdfs:subClassOf ns1:AdEvent ;
    skos:definition "User interaction with an advertisement" .

ns1:Impression a owl:Class ;
    rdfs:label "Impression"@en ;
    rdfs:subClassOf ns1:AdEvent ;
    skos:definition "An ad impression shown to a user" .

ns1:InAppPurchase a owl:Class ;
    rdfs:label "In-App Purchase"@en ;
    rdfs:subClassOf ns1:Transaction ;
    skos:altLabel "IAP"@en ;
    skos:definition "A purchase made within a game" .

ns1:InactivePlayer a owl:Class ;
    rdfs:label "Inactive Player"@en ;
    rdfs:subClassOf ns1:PlayerState ;
    skos:definition "Currently inactive player" .

ns1:Person a owl:Class ;
    rdfs:label "New Class"@en ;
    rdfs:subClassOf ns1:Actor ;
    skos:definition "A Human that interacts with a system" .

ns1:belongsToDevice a owl:ObjectProperty ;
    rdfs:label "belongs to device"@en ;
    rdfs:domain <http://ontology.gaming.network/universal/human_behavior#Activity> ;
    rdfs:range ns1:Player ;
    skos:definition "Relates a session to its device" .

ns1:belongsToPlayer a owl:ObjectProperty ;
    rdfs:label "belongs to player"@en ;
    rdfs:domain ns1:GameSession ;
    rdfs:range ns1:Player ;
    skos:definition "Relates a gaming session to the player" .

ns1:occursInSession a owl:ObjectProperty ;
    rdfs:label "occurs in session"@en ;
    rdfs:domain ns1:GameEvent ;
    rdfs:range ns1:GameSession ;
    skos:definition "Relates a gaming event to the session it occurs in" .

<http://ontology.gaming.network/universal/human_behavior> a owl:Ontology ;
    dc:creator "Gi Fernando" ;
    dc:date "2025-12-27" ;
    dc:title "Universal Human Behavior Foundation" ;
    rdfs:comment "Universal extensible foundation for human behavior data across domains" ;
    owl:versionInfo "1.0.0" .

ns1:Actor a owl:Class ;
    rdfs:label "Actor"@en ;
    rdfs:subClassOf ns1:Entity ;
    skos:definition "An entity that can perform actions in the gaming ecosystem" .

ns1:AtRisk a owl:Class ;
    rdfs:label "At Risk"@en ;
    rdfs:subClassOf ns1:RetentionStatus ;
    skos:definition "User who may churn soon" .

ns1:AttributedInstall a owl:Class ;
    rdfs:label "Attributed Install"@en ;
    rdfs:subClassOf <http://ontology.gaming.network/universal/human_behavior#BehavioralEvent> ;
    skos:definition "A game installation attributed to a campaign" .

ns1:Bid a owl:Class ;
    rdfs:label "Bid"@en ;
    rdfs:subClassOf ns1:AdEvent ;
    skos:definition "A bid request in the ad auction" .

ns1:Churned a owl:Class ;
    rdfs:label "Churned"@en ;
    rdfs:subClassOf ns1:RetentionStatus ;
    skos:definition "User who has not returned after first session" .

ns1:Dolphin a owl:Class ;
    rdfs:label "Dolphin"@en ;
    rdfs:subClassOf ns1:MonetizationSegment ;
    skos:definition "User with medium spending",
        "User with medium spending (£10-£50)" .

ns1:HighEngagement a owl:Class ;
    rdfs:label "High Engagement"@en ;
    rdfs:subClassOf ns1:EngagementLevel ;
    skos:definition "User with high engagement (10+ sessions)" .

ns1:LowEngagement a owl:Class ;
    rdfs:label "Low Engagement"@en ;
    rdfs:subClassOf ns1:EngagementLevel ;
    skos:definition "User with low engagement (1-2 sessions)" .

ns1:MediumEngagement a owl:Class ;
    rdfs:label "Medium Engagement"@en ;
    rdfs:subClassOf ns1:EngagementLevel ;
    skos:definition "User with medium engagement (3-9 sessions)" .

ns1:Minnow a owl:Class ;
    rdfs:label "Minnow"@en ;
    rdfs:subClassOf ns1:MonetizationSegment ;
    skos:definition "User with low spending",
        "User with low spending (£0-£10)" .

ns1:NonPayer a owl:Class ;
    rdfs:label "Non-Payer"@en ;
    rdfs:subClassOf ns1:MonetizationSegment ;
    skos:definition "User who has never made a purchase" .

ns1:PlayerState a owl:Class ;
    rdfs:label "Player State"@en ;
    rdfs:comment "Extends universal BehavioralState for player state classification." ;
    rdfs:subClassOf <http://ontology.gaming.network/universal/human_behavior#BehavioralState> ;
    skos:definition "Current player state (Active, Inactive, Churned)" .

ns1:Retained a owl:Class ;
    rdfs:label "Retained"@en ;
    rdfs:subClassOf ns1:RetentionStatus ;
    skos:definition "User who continues to engage regularly" .

ns1:Whale a owl:Class ;
    rdfs:label "Whale"@en ;
    rdfs:subClassOf ns1:MonetizationSegment ;
    skos:definition "User with high spending",
        "User with high spending (£50+)" .

ns1:Transaction a owl:Class ;
    rdfs:label "Transaction"@en ;
    rdfs:subClassOf <http://ontology.gaming.network/universal/human_behavior#BehavioralEvent> ;
    skos:definition "A financial transaction" .

ns1:AdEvent a owl:Class ;
    rdfs:label "Ad Event"@en ;
    rdfs:subClassOf <http://ontology.gaming.network/universal/human_behavior#BehavioralEvent> ;
    skos:definition "An event related to advertising" .

ns1:Campaign a owl:Class ;
    rdfs:label "Campaign"@en ;
    rdfs:subClassOf ns1:Entity ;
    skos:definition "An advertising campaign" .

ns1:EngagementLevel a owl:Class ;
    rdfs:label "Engagement Level"@en ;
    rdfs:comment "Extends universal BehavioralState for engagement classification." ;
    rdfs:subClassOf ns1:Entity,
        <http://ontology.gaming.network/universal/human_behavior#BehavioralState> ;
    skos:definition "Classification of user engagement" .

ns1:MonetizationEvent a owl:Class ;
    rdfs:label "Monetization Event"@en ;
    rdfs:comment "Events related to monetization and revenue generation." ;
    rdfs:subClassOf ns1:GameEvent ;
    skos:definition "Monetization-related events (Purchase, IAP, Subscription)" .

ns1:RetentionStatus a owl:Class ;
    rdfs:label "Retention Status"@en ;
    rdfs:comment "Extends universal BehavioralState for retention classification." ;
    rdfs:subClassOf ns1:Entity,
        <http://ontology.gaming.network/universal/human_behavior#BehavioralState> ;
    skos:definition "Classification of user retention" .

ns1:MonetizationSegment a owl:Class ;
    rdfs:label "Monetization Segment"@en ;
    rdfs:comment "Extends universal BehavioralState for monetization segmentation." ;
    rdfs:subClassOf ns1:Entity,
        <http://ontology.gaming.network/universal/human_behavior#BehavioralState> ;
    skos:definition "Classification of user monetization behavior" .

ns1:EngagementEvent a owl:Class ;
    rdfs:label "Engagement Event"@en ;
    rdfs:comment "Events related to player engagement and progression." ;
    rdfs:subClassOf ns1:GameEvent ;
    skos:definition "Engagement-related events (LevelStart, LevelComplete, Achievement)" .

ns1:Game a owl:Class ;
    rdfs:label "Game"@en ;
    rdfs:comment "Represents a game application." ;
    rdfs:subClassOf ns1:Entity ;
    skos:definition "A game application in the network",
        "Game application" .

ns1:GameSession a owl:Class ;
    rdfs:label "Game Session"@en ;
    rdfs:comment "Represents a gaming session, extending universal Activity concept." ;
    rdfs:subClassOf <http://ontology.gaming.network/universal/human_behavior#Activity> ;
    skos:definition "A session within a specific game",
        "Gaming activity period" .

ns1:MonetizationThresholds a owl:Class ;
    rdfs:label "Monetization Thresholds"@en ;
    rdfs:subClassOf ns1:Entity ;
    skos:definition "Configuration class for tenant-specific monetization segment thresholds"@en .

ns1:Entity a owl:Class ;
    rdfs:label "Entity"@en ;
    skos:definition "Top-level class for all entities in the gaming ecosystem" .

ns1:GameEvent a owl:Class ;
    rdfs:label "Game Event"@en ;
    rdfs:comment "Base class for all gaming events, extending universal BehavioralEvent." ;
    rdfs:subClassOf <http://ontology.gaming.network/universal/human_behavior#BehavioralEvent> ;
    skos:definition "Gaming-specific events" .

<http://ontology.gaming.network/universal/human_behavior#BehavioralState> a owl:Class ;
    rdfs:label "Behavioral State"@en ;
    rdfs:comment "Base class for any behavioral state. Extensible to domain-specific states." ;
    skos:definition "Universal concept for any behavioral state (Engagement, Recovery, MarketState, VideoEmotionState)" .

<http://ontology.gaming.network/universal/human_behavior#HumanActor> a owl:Class ;
    rdfs:label "Human Actor"@en ;
    rdfs:comment "Base class for any human actor in behavioral data. Extensible to domain-specific actors." ;
    skos:definition "Universal concept for any human entity (Player, Patient, Trader, Consumer, VideoSubject)" .

<http://ontology.gaming.network/universal/human_behavior#BehavioralEvent> a owl:Class ;
    rdfs:label "Behavioral Event"@en,
        "Event"@en ;
    rdfs:comment "Base class for any behavioral event. Extensible to domain-specific events." ;
    rdfs:subClassOf ns1:Entity ;
    skos:definition "A temporal occurrence in the gaming ecosystem",
        "Universal concept for any behavioral event (Purchase, Treatment, Movement, VideoAction, Trade)" .

<http://ontology.gaming.network/universal/human_behavior#Activity> a owl:Class ;
    rdfs:label "Activity"@en,
        "Session"@en ;
    rdfs:comment "Base class for any activity period. Extensible to domain-specific activities." ;
    rdfs:subClassOf <http://ontology.gaming.network/universal/human_behavior#BehavioralEvent> ;
    skos:definition "A period of continuous interaction with a game",
        "Universal concept for any human activity (GameSession, TreatmentSession, VideoPlaythrough, TradingSession)" .

ns1:Player a owl:Class ;
    rdfs:label "Device"@en,
        "Player"@en ;
    ns1:businessDefinition "A tracked entity representing a player/device from a business perspective."@en ;
    ns1:businessRationale "We need this definition for client-facing documentation and alignment."@en ;
    ns1:businessTerms "player, user, device"@en ;
    ns1:businessThreshold "N/A"@en ;
    ns1:businessUseCase "Segmentation, retention analysis, client mapping"@en ;
    ns1:contributedBy "test_user" ;
    rdfs:comment "Represents a player/user in gaming context. Alias for Device/User terminology.",
        "Represents the same concept as Player or User in different games" ;
    rdfs:subClassOf ns1:Actor,
        <http://ontology.gaming.network/universal/human_behavior#HumanActor> ;
    skos:altLabel "Device"@en,
        "Player"@en,
        "User"@en ;
    skos:definition "A unique hardware device used to access games",
        "Gaming-specific human actor" .

[] a owl:AllDisjointClasses ;
    owl:members ( <http://ontology.gaming.network/universal/human_behavior#HumanActor> <http://ontology.gaming.network/universal/human_behavior#Activity> <http://ontology.gaming.network/universal/human_behavior#BehavioralEvent> <http://ontology.gaming.network/universal/human_behavior#BehavioralState> ) .

[] a owl:AllDisjointClasses ;
    owl:members ( ns1:HighEngagement ns1:MediumEngagement ns1:LowEngagement ) .

[] a owl:AllDisjointClasses ;
    owl:members ( ns1:Retained ns1:AtRisk ns1:Churned ) .

[] a owl:AllDisjointClasses ;
    owl:members ( ns1:ActivePlayer ns1:InactivePlayer ) .

[] a owl:AllDisjointClasses ;
    owl:members ( ns1:Whale ns1:Dolphin ns1:Minnow ns1:NonPayer ) .

[] a owl:AllDisjointClasses ;
    owl:members ( <http://ontology.gaming.network/universal/human_behavior#HumanActor> <http://ontology.gaming.network/universal/human_behavior#Activity> <http://ontology.gaming.network/universal/human_behavior#BehavioralEvent> <http://ontology.gaming.network/universal/human_behavior#BehavioralState> ) .

[] a owl:AllDisjointClasses ;
    owl:members ( ns1:Retained ns1:AtRisk ns1:Churned ) .

[] a owl:AllDisjointClasses ;
    owl:members ( ns1:ActivePlayer ns1:InactivePlayer ) .

[] a owl:AllDisjointClasses ;
    owl:members ( ns1:Whale ns1:Dolphin ns1:Minnow ns1:NonPayer ) .

[] a owl:AllDisjointClasses ;
    owl:members ( ns1:HighEngagement ns1:MediumEngagement ns1:LowEngagement ) .

